Fix triple for lazy list creation

lazy_list/spec.v
@@ -3,65 +3,76 @@ From iris.base_logic.lib Require Export invariants.
 
 From SkipList.lazy_list Require Import code.
 
-From Coq Require Import Lists.ListSet.
-
 Local Open Scope Z.
 Module LazyListSpec (Params: LAZYLIST_PARAMS).
   Import Params.
   Module Code := Lazylist Params.
   Export Code.
 
-Context `{!heapGS Σ} (N : namespace).
+  Context `{!heapGS Σ} (N : namespace).
 
-Fixpoint list_equiv (L: list Z) (node: val) : iProp Σ :=
-  match L with
-  | nil => ⌜ node = NONEV ⌝
-  | h :: t => ∃ (k: Z) (n: loc) (m: bool) (l: val) (v': val) (γ: gname),
-              ⌜ node = rep_to_node (k, n, m, l) ⌝
-              ∗
-              ⌜ k = h ⌝
-              ∗
-              n ↦ v'
-              ∗
-              (* is_lock γ l ???
-              ∗ *)
-              list_equiv t v'
-  end.
+  (* 
+  * The sequence of keys must be the same and
+  * the lock invariant must hold in all nodes.
+  *)
+  Fixpoint list_equiv (L: list Z) (node: val) : iProp Σ :=
+    match L with
+    | nil => ⌜ node = NONEV ⌝
+    | h :: t => ∃ (k: Z) (n: loc) (m: bool) (l: val) (v': val) (γ: gname),
+                ⌜ node = rep_to_node (k, n, m, l) ⌝
+                ∗
+                ⌜ k = h ⌝
+                ∗
+                n ↦ v'
+                ∗
+                (* is_lock γ l ???
+                ∗ *)
+                ▷list_equiv t v'
+    end.
 
-Definition lazy_list_inv (S: set Z) (l: loc) : iProp Σ := 
-  ∃ (L: list Z) (head: val),
-  (* ⌜ Permutation L (elements S) ⌝
-  ∗ *)
-  (* ⌜ Sorted Zlt L ⌝
-  ∗ *)
-  l ↦ head
-  ∗
-  list_equiv L head
-.
-
-Definition is_lazy_list (S: set Z) (l: loc) : iProp Σ := 
-  inv N (lazy_list_inv S l).
-
-Definition empty_lazy := [INT_MIN; INT_MAX].
-
-Theorem new_spec :
-  {{{ True }}}
-    new #()
-  {{{ l, RET l; 
-    is_lazy_list empty_lazy l 
-  }}}.
-Proof.
-Admitted.
-
-Theorem contains_spec (S: set Z) (l: loc) (key: Z) :
-  {{{ is_lazy_list S l }}}
-    contains !#l #key
-  {{{ b, RET b; 
-    is_lazy_list S l
+  (* 
+  * The invariant for the lazy list asserts that
+  * the underlying set S is sorted and must contain
+  * the same elements as S.
+  *)
+  Definition lazy_list_inv (S: gset Z) (l: loc) : iProp Σ := 
+    ∃ (L: list Z) (head: val),
+    ⌜ Permutation L (elements S) ⌝
     ∗
-    ⌜ (b = False ∧ ¬ key ∈ S)
-    ∨
-    (b = True ∧ key ∈ S) ⌝
-  }}}.
-Proof.
-Admitted.
+    (* ⌜ Sorted Zlt L ⌝
+    ∗ *)
+    l ↦ head
+    ∗
+    list_equiv ([INT_MIN] ++ L ++ [INT_MAX]) head
+  .
+
+  (* 
+  * Asserts that l points to a heap cell that 
+  * represents the set S as a lazy list.
+  *)
+  Definition is_lazy_list (S: gset Z) (v: val) : iProp Σ := 
+    ∃ (l: loc), ⌜v = #l⌝ ∗ inv N (lazy_list_inv S l).
+
+  Theorem new_spec (S: gset Z) :
+    {{{ True }}}
+      new #()
+    {{{ (v: val), RET v; 
+      is_lazy_list ∅ v 
+    }}}.
+  Proof.
+  Admitted.
+
+  (* Theorem contains_spec (S: gset Z) (v: val) (key: Z) :
+    {{{ is_lazy_list S v }}}
+      contains !v #key
+    {{{ (b: bool), RET b; 
+      is_lazy_list S v
+      ∗
+      ⌜ (b = false ∧ ¬ key ∈ S)
+      ∨
+      (b = true ∧ key ∈ S) ⌝
+    }}}.
+  Proof.
+  Admitted. *)
+
+End LazyListSpec.
